---
permalink: /.ttl
---
@prefix cs: <https://linked.data.gov.au/def/supermodel/terms> .
@prefix rdf:  <http://www.w3.org/1999/02/22-rdf-syntax-ns#> .
@prefix rdfs: <http://www.w3.org/2000/01/rdf-schema#> .
@prefix owl:  <http://www.w3.org/2002/07/owl#> .
@prefix xsd:  <http://www.w3.org/2001/XMLSchema#> .
@prefix sdo: <https://schema.org/> .
@prefix skos: <http://www.w3.org/2004/02/skos/core#> .
@prefix reg:  <http://purl.org/linked-data/registry#> .
@prefix dcterms:  <http://purl.org/dc/terms/> .
@prefix : <https://linked.data.gov.au/def/supermodel/terms/> .


<https://linked.data.gov.au/def/supermodel/terms> 
    a owl:Ontology , skos:ConceptScheme ;
    dcterms:identifier "supermodel-terms"^^xsd:token ;
    skos:prefLabel "Supermodel Terms Vocabulary"@en ;
    skos:definition """This repository contains a Semantic Web vocabulary that defines terms of the Supermodel data model. The vocabulary is available online in human- and machine-readable form at: https://linked.data.gov.au/def/supermodel/terms."""@en ;
    owl:versionIRI <https://linked.data.gov.au/def/supermodel/terms/1.0> ;
    owl:versionInfo "1.0"@en ;
    dcterms:contributor <https://orcid.org/0000-0002-8742-7730>;
    dcterms:creator <http://orcid.org/0000-0002-8742-7730> ;
    dcterms:publisher <https://linked.data.gov.au/org/agldwg> ;
    rdfs:seeAlso <https://github.com/agldwg/supermodel-terms-vocab> ;
    dcterms:issued "2022-04-12"^^xsd:date ;
    dcterms:modified "2022-04-12"^^xsd:date ;
    dcterms:rights "(c) Commonwealth of Australia (Australian Government Linked Data Working Group), 2022"@en ;
    dcterms:created "2022-04-12"^^xsd:date ;
    dcterms:source "https://linked.data.gov.au/def/supermodel"^^xsd:anyURI ;
    skos:hasTopConcept 
        <https://linked.data.gov.au/def/supermodel/terms/central-class> ,
        <https://linked.data.gov.au/def/supermodel/terms/data-domain> ,
        <https://linked.data.gov.au/def/supermodel/terms/knowledge-graph> ,
        <https://linked.data.gov.au/def/supermodel/terms/linked-data> ,
        <https://linked.data.gov.au/def/supermodel/terms/semantic-web> ;
.

<https://linked.data.gov.au/def/agldwg>
    a sdo:Organization ;
    sdo:name "Australian government Linked Data Working Group" ;
    sdo:url "https://linked.data.gov.au"^^xsd:anyURI ;
.

<https://orcid.org/0000-0002-8742-7730>
    a sdo:Person ;
    sdo:honorificPrefix "Dr" ;
    sdo:name "Nicholas J. Car" ;
    sdo:email "nicholas.car@surroundaustralia.com"^^xsd:anyURI ;
    sdo:affiliation <https://linked.data.gov.au/org/surround> ;
.

<https://linked.data.gov.au/def/supermodel/terms/central-class>
    a skos:Concept ;
    dcterms:identifier "central-class"^^xsd:token ;
    rdfs:isDefinedBy cs: ;
    skos:prefLabel "Central Class"@en ;
    skos:definition """Central Classes are the generic data classes at the centre of Data Domains with high-level relationships between them defined in this supermodel.

These classes are taken from general standards - usually well-known international stadnards - and Geoscience Australia specialises and extends them to make specific, custom, classes for their needs."""@en ;
    skos:inScheme cs: ;
    skos:topConceptOf cs: ;
    dcterms:provenance "Defined within the Supermodel model" ;
.

<https://linked.data.gov.au/def/supermodel/terms/data-domain>
    a skos:Concept ;
    dcterms:identifier "data-domain"^^xsd:token ;
    rdfs:isDefinedBy cs: ;
    skos:prefLabel "Data Domain"@en ;
    skos:definition """High-level conceptual areas within which a supermodel has data."""@en ;
    skos:scopeNote """Data Domains are not themed at a level above science domains or domains within other, particular, diciplines but are instead based on parts of measurement models, such as the Observations & Measurement ISO19156 standard. This is to ensure that the domains are relevant to many forms of data, given that data is often measured and observed."""@en ;
    skos:inScheme cs: ;
    skos:topConceptOf cs: ;
    dcterms:provenance "Defined within the Supermodel model" ;
.

<https://linked.data.gov.au/def/supermodel/terms/knowledge-graph>
    a skos:Concept ;
    dcterms:identifier "knowledge-graph"^^xsd:token ;
    rdfs:isDefinedBy cs: ;
    skos:prefLabel "Knowledge Graph"@en ;
    skos:definition """A Knowledge Graph is a dataset that uses a graph data tructure - nodes and edges - with strongly-defined elements."""@en ;
    skos:inScheme cs: ;
    skos:topConceptOf cs: ;
    dcterms:provenance "Defined within the Supermodel model" ;
.

<https://linked.data.gov.au/def/supermodel/terms/linked-data>
    a skos:Concept ;
    dcterms:identifier "linked-data"^^xsd:token ;
    rdfs:isDefinedBy cs: ;
    skos:prefLabel "Linked Data"@en ;
    skos:definition """A set of technologies and conventions defined by the World Wide Web Consortium that aim to present data in both human- and machine-readable form over the Internet.

Linked Data is strongly-defined with each element having either a local definition or a link to an available definition on the Internet.

Linked Data is graph-based in nature, that is it consistes of nodes and edges that can forever be linked to further conceps with defined relationships."""@en ;
    dcterms:source "https://www.w3.org/standards/semanticweb/data"^^xsd:anyURI ;
    skos:inScheme cs: ;
    skos:topConceptOf cs: ;
    dcterms:provenance "Defined within the Supermodel model" ;
.

<https://linked.data.gov.au/def/supermodel/terms/semantic-web>
    a skos:Concept ;
    dcterms:identifier "semantic-web"^^xsd:token ;
    rdfs:isDefinedBy cs: ;
    skos:prefLabel "Semantic Web"@en ;
    skos:definition """The World Wide Web Consortium's vision of an Internet-based web of Linked Data.

Semantic Web is used to refer to something more than just the technologies and conventions of Linked Data; the term also encompases a specific set of interoperable data models - often called ontologies - published by the W3C, other standards bodies and some well-known companies.

The 'semantic' refers to the strongly-defined nature of the elements in the Semantic Web: the meaning of Semantic Web data is as precicely defined as any data can be."""@en ;
    dcterms:source "https://www.w3.org/standards/semanticweb/"^^xsd:anyURI ;
    skos:inScheme cs: ;
    skos:topConceptOf cs: ;
    dcterms:provenance "Defined within the Supermodel model" ;
.
