---
permalink: /.ttl
---
@prefix cs: <https://linked.data.gov.au/def/supermodel/terms> .
@prefix rdf:  <http://www.w3.org/1999/02/22-rdf-syntax-ns#> .
@prefix rdfs: <http://www.w3.org/2000/01/rdf-schema#> .
@prefix owl:  <http://www.w3.org/2002/07/owl#> .
@prefix xsd:  <http://www.w3.org/2001/XMLSchema#> .
@prefix sdo: <https://schema.org/> .
@prefix skos: <http://www.w3.org/2004/02/skos/core#> .
@prefix reg:  <http://purl.org/linked-data/registry#> .
@prefix dcterms:  <http://purl.org/dc/terms/> .
@prefix : <https://linked.data.gov.au/def/supermodel/terms/> .


<https://linked.data.gov.au/def/supermodel/terms> 
    a owl:Ontology , skos:ConceptScheme ;
    dcterms:identifier "supermodel-terms"^^xsd:token ;
    skos:prefLabel "Supermodel Terms Vocabulary"@en ;
    skos:definition """This repository contains a Semantic Web vocabulary that defines terms of the Supermodel data model. The vocabulary is available online in human- and machine-readable form at: https://linked.data.gov.au/def/supermodel/terms."""@en ;
    owl:versionIRI <https://linked.data.gov.au/def/supermodel/terms/1.0> ;
    owl:versionInfo "1.0"@en ;
    dcterms:contributor <https://orcid.org/0000-0002-8742-7730>;
    dcterms:creator <http://orcid.org/0000-0002-8742-7730> ;
    dcterms:publisher <https://linked.data.gov.au/org/agldwg> ;
    rdfs:seeAlso <https://github.com/agldwg/supermodel-terms-vocab> ;
    dcterms:issued "2022-04-14"^^xsd:date ;
    dcterms:modified "2022-04-12"^^xsd:date ;
    dcterms:rights "(c) Commonwealth of Australia (Australian Government Linked Data Working Group), 2022"@en ;
    dcterms:created "2022-04-12"^^xsd:date ;
    dcterms:source "https://linked.data.gov.au/def/supermodel"^^xsd:anyURI ;
    skos:hasTopConcept 
        <https://linked.data.gov.au/def/supermodel/terms/backbone-model> ,
        <https://linked.data.gov.au/def/supermodel/terms/background-model> ,
        <https://linked.data.gov.au/def/supermodel/terms/central-class> ,
        <https://linked.data.gov.au/def/supermodel/terms/data-domain> ,
        <https://linked.data.gov.au/def/supermodel/terms/knowledge-graph> ,
        <https://linked.data.gov.au/def/supermodel/terms/linked-data> ,
        <https://linked.data.gov.au/def/supermodel/terms/semantic-web> ,
        <https://linked.data.gov.au/def/supermodel/terms/vocabulary> ;
.

<https://linked.data.gov.au/def/supermodel/terms/backbone-model>
    a skos:Concept ;
    rdfs:isDefinedBy cs: ;
    skos:prefLabel "Backbone Model"@en ;
    skos:definition """An integrative, summary model, that allows for crosswalking of elements within the Component Models of a Supermodel."""@en ;
    skos:inScheme cs: ;
    skos:topConceptOf cs: ;
.

<https://linked.data.gov.au/def/supermodel/terms/background-model>
    a skos:Concept ;
    rdfs:isDefinedBy cs: ;
    skos:prefLabel "Background Model"@en ;
    skos:definition """A standard and common Semantic Web model used as "upper" or higher order/abstract model for all other Supermodel models to conform to when modelling something within the Background Model's purview."""@en ;
    skos:inScheme cs: ;
    skos:topConceptOf cs: ;
.

<https://linked.data.gov.au/def/agldwg>
    a sdo:Organization ;
    sdo:name "Australian government Linked Data Working Group" ;
    sdo:url "https://linked.data.gov.au"^^xsd:anyURI ;
.

<https://orcid.org/0000-0002-8742-7730>
    a sdo:Person ;
    sdo:honorificPrefix "Dr" ;
    sdo:name "Nicholas J. Car" ;
    sdo:email "nicholas.car@surroundaustralia.com"^^xsd:anyURI ;
    sdo:affiliation <https://linked.data.gov.au/org/surround> ;
.

<https://linked.data.gov.au/def/supermodel/terms/central-class>
    a skos:Concept ;
    dcterms:identifier "central-class"^^xsd:token ;
    rdfs:isDefinedBy cs: ;
    skos:prefLabel "Central Class"@en ;
    skos:definition """Central Classes are the generic data classes at the centre of Data Domains with high-level relationships between them defined in this supermodel.

These classes are taken from general standards - usually well-known international standards - and they are specialised and extended within Supermodel implementations as needed."""@en ;
    skos:inScheme cs: ;
    skos:topConceptOf cs: ;
    dcterms:provenance "Defined within the Supermodel model" ;
.

<https://linked.data.gov.au/def/supermodel/terms/data-domain>
    a skos:Concept ;
    dcterms:identifier "data-domain"^^xsd:token ;
    rdfs:isDefinedBy cs: ;
    skos:prefLabel "Data Domain"@en ;
    skos:definition """High-level conceptual areas within which a supermodel has data."""@en ;
    skos:scopeNote """Data Domains are not themed at a level above science domains or domains within other, particular, diciplines but are instead based on parts of measurement models, such as the Observations & Measurement ISO19156 standard. This is to ensure that the domains are relevant to many forms of data, given that data is often measured and observed."""@en ;
    skos:inScheme cs: ;
    skos:topConceptOf cs: ;
    dcterms:provenance "Defined within the Supermodel model" ;
.

<https://linked.data.gov.au/def/supermodel/terms/knowledge-graph>
    a skos:Concept ;
    dcterms:identifier "knowledge-graph"^^xsd:token ;
    rdfs:isDefinedBy cs: ;
    skos:prefLabel "Knowledge Graph"@en ;
    skos:definition """A Knowledge Graph is a dataset that uses a graph data tructure - nodes and edges - with strongly-defined elements."""@en ;
    skos:inScheme cs: ;
    skos:topConceptOf cs: ;
    dcterms:provenance "Defined within the Supermodel model" ;
.

<https://linked.data.gov.au/def/supermodel/terms/linked-data>
    a skos:Concept ;
    dcterms:identifier "linked-data"^^xsd:token ;
    rdfs:isDefinedBy cs: ;
    skos:prefLabel "Linked Data"@en ;
    skos:definition """A set of technologies and conventions defined by the World Wide Web Consortium that aim to present data in both human- and machine-readable form over the Internet.

Linked Data is strongly-defined with each element having either a local definition or a link to an available definition on the Internet.

Linked Data is graph-based in nature, that is it consistes of nodes and edges that can forever be linked to further conceps with defined relationships."""@en ;
    dcterms:source "https://www.w3.org/standards/semanticweb/data"^^xsd:anyURI ;
    skos:inScheme cs: ;
    skos:topConceptOf cs: ;
    dcterms:provenance "Defined within the Supermodel model" ;
.

<https://linked.data.gov.au/def/supermodel/terms/location-index>
    a skos:Concept ;
    rdfs:isDefinedBy cs: ;
    skos:prefLabel "Location Index"@en ;
    skos:definition """A project undertaken by CSIRO, Geoscience Australia and other Australin government organisations from 2018 onwards aiming to provide a consistent way to seamlessly integrate spatial data from distributed sources."""@en ;
    skos:inScheme cs: ;
    skos:topConceptOf cs: ;
    dcterms:source "http://www.ga.gov.au/locationindex"^^xsd:anyURI ;
.

<https://linked.data.gov.au/def/supermodel/terms/ontology>
    a skos:Concept ;
    rdfs:isDefinedBy cs: ;
    skos:prefLabel "Ontology"@en ;
    skos:definition """In computer science and information science, an ontology encompasses a representation, formal naming, and definition of the categories, properties, and relations between the concepts, data, and entities that substantiate one, many, or all domains of discourse.

The word ontology was originally defined as "the branch of philosophy that studies concepts such as existence, being, becoming, and reality". and the computer science term is derived from that definition."""@en ;
    skos:inScheme cs: ;
    skos:topConceptOf cs: ;
    dcterms:provenance "This definition was created for this vocabulary based on several sources, in particular Semantic Web web pages from the W3C (see 'Semantic Web') and Wikipedia's Ontology (Computer Science) page" ;
.

<https://linked.data.gov.au/def/supermodel/terms/semantic-web>
    a skos:Concept ;
    dcterms:identifier "semantic-web"^^xsd:token ;
    rdfs:isDefinedBy cs: ;
    skos:prefLabel "Semantic Web"@en ;
    skos:definition """The World Wide Web Consortium's vision of an Internet-based web of Linked Data.

Semantic Web is used to refer to something more than just the technologies and conventions of Linked Data; the term also encompases a specific set of interoperable data models - often called ontologies - published by the W3C, other standards bodies and some well-known companies.

The 'semantic' refers to the strongly-defined nature of the elements in the Semantic Web: the meaning of Semantic Web data is as precicely defined as any data can be."""@en ;
    dcterms:source "https://www.w3.org/standards/semanticweb/"^^xsd:anyURI ;
    skos:inScheme cs: ;
    skos:topConceptOf cs: ;
    dcterms:provenance "Defined within the Supermodel model" ;
.

<https://linked.data.gov.au/def/supermodel/terms/vocabulary>
    a skos:Concept ;
    rdfs:isDefinedBy cs: ;
    skos:prefLabel "Vocabulary"@en ;
    skos:definition """A managed codelist or taxonomy of concepts."""@en ;
    skos:scopeNote "Supermodels tend to use vocabularies formulated according to the SKOS (https://www.w3.org/TR/skos-reference/) or lists of objects defined using basic RDF (http://www.w3.org/TR/rdf11-concepts/), RDFS (https://www.w3.org/TR/rdf-schema/) or OWL (https://www.w3.org/TR/owl2-overview/) elements."@en ;
    skos:inScheme cs: ;
    skos:topConceptOf cs: ;
.
